A roughly complete formalization of (multi)sets.

MultiSet/MultiSet.v
@@ -1,29 +1,248 @@
-Require Import Lists.List OrdType Bool SortedList.
+Require Import Lists.List OrdType Bool SortedList JMeq Omega.
+
+Notation " x ~= y " := (@JMeq _ x _ y) (at level 70, no associativity).
+
+Lemma eq_JMeq {A} {x y : A} (H : x = y) : x ~= y.
+Proof.
+  rewrite H. reflexivity.
+Qed.
+
 
 Module MultiSet (O : OrdType.OrdType).
   Module S := InsertionSort O.
   Import S.
 
+  (* the type of sets *)
   Definition t := { l : list O.t & is_sorted l = true }.
 
-  Print Orders.OrderedTypeFull.
+  (* some basic list operations *)
+  Definition list_minus : list O.t -> list O.t -> list O.t
+    := fun l1 l2 => 
+      let l := nodup O.eq_dec (l1 ++ l2) in
+      fold_left (fun acc x => acc ++ repeat x (count_occ O.eq_dec l1 x - count_occ O.eq_dec l2 x)) l List.nil.
+  Definition list_inter : list O.t -> list O.t -> list O.t
+    := fun l1 l2 => 
+      let l := nodup O.eq_dec (l1 ++ l2) in
+      fold_left (fun acc x => acc ++ repeat x (min (count_occ O.eq_dec l1 x) (count_occ O.eq_dec l2 x))) l List.nil.
 
   (* multiset operations *)
   Definition memb   : O.t -> t -> nat
     := fun x A => List.count_occ O.eq_dec (projT1 A) x.
   Definition plus   : t -> t -> t
     := fun A B => existT _ (sort (projT1 A ++ projT1 B)) (sort_is_sorted _).
-  Parameter minus   : t -> t -> t.
-  Parameter inter   : t -> t -> t.
-  Parameter set_of  : t -> t.
-  Parameter of_list : list O.t -> t.
+  Definition minus   : t -> t -> t
+    := fun A B => 
+      let l := nodup O.eq_dec (projT1 A ++ projT1 B) in
+      let l' := fold_left (fun acc x => acc ++ repeat x (min (memb x A) (memb x B))) l List.nil in
+      existT _ (sort (list_minus (projT1 A) (projT1 B))) (sort_is_sorted _).
+  Definition inter   : t -> t -> t
+    := fun A B => 
+      let l := nodup O.eq_dec (projT1 A ++ projT1 B) in
+      let l' := fold_left (fun acc x => acc ++ repeat x (min (memb x A) (memb x B))) l List.nil in
+      existT _ (sort (list_inter (projT1 A) (projT1 B))) (sort_is_sorted _).
+  Definition set_of  : t -> t
+    := fun A => existT _ (sort (nodup O.eq_dec (projT1 A))) (sort_is_sorted _).
+  Definition of_list : list O.t -> t
+    := fun l => existT _ (sort l) (sort_is_sorted _).
 
+  (* auxiliary lemma *)
+  Lemma existT_eq A (f : A -> Type) x x' e e' : x ~= x' -> e ~= e' -> existT f x e ~= existT f x' e'.
+  Proof.
+    intro. generalize e; clear e. rewrite H. intros. rewrite H0. reflexivity.
+  Qed.
 
-  (* properties *)
-  Parameter p_ext : forall A B, (forall t, memb t A = memb t B) -> A = B.
-  Parameter p_plus : forall A B, forall t, memb t (plus A B) = memb t A + memb t B.
-  Parameter p_minus : forall A B, forall t, memb t (minus A B) = memb t A - memb t B.
-  Parameter p_inter : forall A B, forall t, memb t (inter A B) = min (memb t A) (memb t B).
-  Parameter p_set_of : forall A, forall t, 0 < memb t A <-> memb t (set_of A) = 1.
+  (***********************************************************************************************)
+  (* PROPERTIES *)
+
+  (* extensional equality *)
+  Lemma p_ext : forall A B, (forall t, memb t A = memb t B) -> A = B.
+  Proof.
+    intros. destruct A. destruct B. unfold memb in H. simpl in H.
+
+    assert (x = x0). 
+    apply ext_eq. apply sorted_is_sorted; assumption. apply sorted_is_sorted; assumption. exact H.
+
+    generalize e; clear e. rewrite H0. intros. f_equal.
+    destruct e. apply JMeq_eq. destruct e0. reflexivity.
+  Qed.
+
+  (* some basic properties of count_occ *)
+  Lemma count_occ_repeat x n : count_occ O.eq_dec (repeat x n) x = n.
+  Proof.
+    induction n; simpl; intuition. destruct (O.eq_dec x x); intuition.
+  Qed.
+
+  Lemma count_occ_repeat_neq x y n : x <> y -> count_occ O.eq_dec (repeat x n) y = 0.
+  Proof.
+    intro. induction n; simpl; intuition. destruct (O.eq_dec x y); intuition.
+  Qed.
+
+  Lemma count_occ_app l1 l2 x :
+    count_occ O.eq_dec (l1 ++ l2) x = count_occ O.eq_dec l1 x + count_occ O.eq_dec l2 x.
+  Proof.
+    induction l1; intuition.
+    simpl. destruct (O.eq_dec a x); intuition.
+  Qed.
+
+  Lemma count_occ_fold l1 l2 f l:
+    forall acc, NoDup l -> 
+    (forall x, (0 < count_occ O.eq_dec l1 x \/ 0 < count_occ O.eq_dec l2 x) -> count_occ O.eq_dec l x = 0 -> count_occ O.eq_dec acc x = f x) ->
+    (forall x, (0 < count_occ O.eq_dec l1 x \/ 0 < count_occ O.eq_dec l2 x) -> 0 < count_occ O.eq_dec l x -> count_occ O.eq_dec acc x = 0) ->
+    forall x, (0 < count_occ O.eq_dec l1 x \/ 0 < count_occ O.eq_dec l2 x) ->
+              count_occ O.eq_dec (fold_left (fun acc' y => acc' ++ repeat y (f y)) l acc) x = f x.
+  Proof.
+    induction l; intuition.
+    + simpl. apply IHl.
+      - inversion H; assumption.
+      - intros. destruct (O.eq_dec a x0). 
+        rewrite e. rewrite count_occ_app. rewrite H1. simpl. rewrite count_occ_repeat. reflexivity.
+        exact H2. rewrite e. simpl. destruct (O.eq_dec x0 x0); intuition.
+        rewrite count_occ_app. rewrite H0. rewrite count_occ_repeat_neq. omega. exact n.
+        exact H2. simpl. destruct (O.eq_dec a x0); intuition.
+      - intros. enough (a <> x0).
+        rewrite count_occ_app. rewrite H1. rewrite count_occ_repeat_neq. reflexivity. exact H5.
+        exact H2. simpl. destruct (O.eq_dec a x0); intuition.
+        inversion H. intro. apply H7. rewrite H9. eapply count_occ_In. exact H4.
+      - left. exact H3.
+    + simpl. apply IHl.
+      - inversion H; assumption.
+      - intros. destruct (O.eq_dec a x0). 
+        rewrite e. rewrite count_occ_app. rewrite H1. simpl. rewrite count_occ_repeat. reflexivity.
+        exact H2. rewrite e. simpl. destruct (O.eq_dec x0 x0); intuition.
+        rewrite count_occ_app. rewrite H0. rewrite count_occ_repeat_neq. omega. exact n.
+        exact H2. simpl. destruct (O.eq_dec a x0); intuition.
+      - intros. enough (a <> x0).
+        rewrite count_occ_app. rewrite H1. rewrite count_occ_repeat_neq. reflexivity. exact H5.
+        exact H2. simpl. destruct (O.eq_dec a x0); intuition.
+        inversion H. intro. apply H7. rewrite H9. eapply count_occ_In. exact H4.
+      - right. exact H3.
+  Qed.
+
+  Lemma count_occ_fold' f l:
+    forall acc,
+    forall x, count_occ O.eq_dec l x = 0 -> count_occ O.eq_dec acc x = 0 ->
+              count_occ O.eq_dec (fold_left (fun acc' y => acc' ++ repeat y (f y)) l acc) x = 0.
+  Proof.
+    induction l; intuition. simpl.
+    apply IHl. simpl in H. destruct (O.eq_dec a x); intuition.
+    rewrite count_occ_app. rewrite H0. rewrite count_occ_repeat_neq. reflexivity.
+    simpl in H. destruct (O.eq_dec a x); intuition.
+  Qed.
+
+  Lemma or_eq_lt_n_O n : n = 0 \/ 0 < n.
+  Proof.
+    destruct (Nat.eq_dec n 0); intuition.
+  Qed.
+
+  Lemma count_occ_nodup l x : count_occ O.eq_dec (nodup O.eq_dec l) x = 1 <-> 0 < count_occ O.eq_dec l x.
+  Proof.
+    induction l; intuition.
+    + simpl in H. discriminate H.
+    + simpl in H1. destruct (in_dec O.eq_dec a l); intuition.
+      simpl. destruct (O.eq_dec a x); intuition.
+      simpl in H1. simpl. destruct (O.eq_dec a x); intuition.
+    + simpl. destruct (in_dec O.eq_dec a l); intuition.
+      apply H0. simpl in H1. destruct (O.eq_dec a x); intuition.
+      rewrite <- e. apply count_occ_In. exact i.
+      simpl. simpl in H1. destruct (O.eq_dec a x); intuition.
+      f_equal. apply count_occ_not_In. intro. apply n.
+      rewrite e. eapply nodup_In. exact H2.
+  Qed.
+
+  Lemma count_occ_nodup_O l x : count_occ O.eq_dec (nodup O.eq_dec l) x = 0 <-> count_occ O.eq_dec l x = 0.
+  Proof.
+    induction l; intuition.
+    + simpl in H1. destruct (in_dec O.eq_dec a l); intuition.
+      enough (count_occ O.eq_dec (nodup O.eq_dec l) a = 1).
+      simpl. destruct (O.eq_dec a x); intuition. rewrite e in H0. rewrite H0 in H. discriminate H.
+      apply NoDup_count_occ'. apply NoDup_nodup. apply nodup_In. exact i.
+      simpl in H1. simpl. destruct (O.eq_dec a x); intuition.
+    + simpl. destruct (in_dec O.eq_dec a l); intuition.
+      simpl in H1. destruct (O.eq_dec a x); intuition.
+      simpl. simpl in H1. destruct (O.eq_dec a x); intuition.
+  Qed.
+
+  (* properties of list_minus and list_inter *)
+  Lemma count_occ_list_minus l1 l2 :
+    forall x, count_occ O.eq_dec (list_minus l1 l2) x
+      = count_occ O.eq_dec l1 x - count_occ O.eq_dec l2 x.
+  Proof.
+    intro. unfold list_minus. 
+    destruct (or_eq_lt_n_O (count_occ O.eq_dec l1 x)).
+    destruct (or_eq_lt_n_O (count_occ O.eq_dec l2 x)).
+    rewrite H, H0. apply count_occ_fold'. apply count_occ_nodup_O.
+    rewrite count_occ_app. rewrite H, H0. reflexivity.
+    reflexivity.
+
+    eapply (count_occ_fold l1 l2 (fun y => count_occ O.eq_dec l1 y - count_occ O.eq_dec l2 y)).
+    apply NoDup_nodup. intros.
+    pose (H3 := proj1 (count_occ_nodup_O _ _) H2); clearbody H3.
+    rewrite count_occ_app in H3. destruct (count_occ O.eq_dec l1 x0); intuition.
+    intros. reflexivity.
+    right. exact H0.
+
+    eapply (count_occ_fold l1 l2 (fun y => count_occ O.eq_dec l1 y - count_occ O.eq_dec l2 y)).
+    apply NoDup_nodup. intros.
+    pose (H2 := proj1 (count_occ_nodup_O _ _) H1); clearbody H2.
+    rewrite count_occ_app in H2. destruct (count_occ O.eq_dec l1 x0); intuition.
+    intros. reflexivity.
+    left. exact H.
+  Qed.
+
+  Lemma count_occ_list_inter l1 l2 :
+    forall x, count_occ O.eq_dec (list_inter l1 l2) x
+      = min (count_occ O.eq_dec l1 x) (count_occ O.eq_dec l2 x).
+  Proof.
+    intro. unfold list_inter. 
+    destruct (or_eq_lt_n_O (count_occ O.eq_dec l1 x)).
+    destruct (or_eq_lt_n_O (count_occ O.eq_dec l2 x)).
+    rewrite H, H0. apply count_occ_fold'. apply count_occ_nodup_O.
+    rewrite count_occ_app. rewrite H, H0. reflexivity.
+    reflexivity.
+
+    eapply (count_occ_fold l1 l2 (fun y => min (count_occ O.eq_dec l1 y) (count_occ O.eq_dec l2 y))).
+    apply NoDup_nodup. intros.
+    pose (H3 := proj1 (count_occ_nodup_O _ _) H2); clearbody H3.
+    rewrite count_occ_app in H3. destruct (count_occ O.eq_dec l1 x0); intuition.
+    intros. reflexivity.
+    right. exact H0.
+
+    eapply (count_occ_fold l1 l2 (fun y => min (count_occ O.eq_dec l1 y) (count_occ O.eq_dec l2 y))).
+    apply NoDup_nodup. intros.
+    pose (H2 := proj1 (count_occ_nodup_O _ _) H1); clearbody H2.
+    rewrite count_occ_app in H2. destruct (count_occ O.eq_dec l1 x0); intuition.
+    intros. reflexivity.
+    left. exact H.
+  Qed.
+
+  (* property of disjoint union multisets *)
+  Lemma p_plus : forall A B, forall t, memb t (plus A B) = memb t A + memb t B.
+  Proof.
+    intros. destruct A. destruct B. unfold memb. simpl.
+    rewrite <- count_occ_sort. apply count_occ_app.
+  Qed.
+
+  (* property of difference multisets *)
+  Lemma p_minus : forall A B, forall t, memb t (minus A B) = memb t A - memb t B.
+  Proof.
+    intros A B x. destruct A. destruct B. unfold memb; simpl.
+    rewrite <- count_occ_sort. apply count_occ_list_minus.
+  Qed.
+
+  (* property of intersection multisets *)
+  Lemma p_inter : forall A B, forall t, memb t (inter A B) = min (memb t A) (memb t B).
+  Proof.
+    intros A B x. destruct A. destruct B. unfold memb; simpl.
+    rewrite <- count_occ_sort. apply count_occ_list_inter.
+  Qed.
+
+  (* property of multiset flattening *)
+  Lemma p_set_of : forall A, forall t, 0 < memb t A <-> memb t (set_of A) = 1.
+  Proof.
+    intros A x. destruct A. unfold memb. unfold set_of. simpl. split; intro.
+    rewrite <- count_occ_sort. apply NoDup_count_occ'. apply NoDup_nodup.
+    apply nodup_In. eapply count_occ_In. exact H.
+    rewrite <- count_occ_sort in H. apply count_occ_nodup. exact H.
+  Qed.
 
 End MultiSet.
