MultiSet/SortedList.v
@@ -40,10 +40,8 @@ Module InsertionSort (O : OrdType.OrdType).
 
   Hint Constructors sorted.
 
-  Axiom sorted_is_sorted : forall l, is_sorted l = true <-> sorted l.
-
   Definition is_a_sorting_algorithm (f: list O.t -> list O.t) :=
-    forall al, (forall x, count_occ x al = count_occ x (f al)) /\ sorted (f al).
+    forall al, (forall x, count_occ O.eq_dec al x = count_occ O.eq_dec (f al) x) /\ sorted (f al).
 
 (** Proof of correctness **)
 
@@ -79,13 +77,125 @@ Module InsertionSort (O : OrdType.OrdType).
     simpl. apply insert_sorted. assumption.
   Qed.
 
-  Axiom sort_is_sorted : forall l, is_sorted (sort l) = true.
-
-  Axiom insertion_sort_correct:  is_a_sorting_algorithm sort.
-(*
+  Lemma le_le_list a t l : O.leb a t = true -> le_list t l = true -> le_list a l = true.
   Proof.
-    split. apply sort_perm. apply sort_sorted.
+    intro. elim l; intuition.
+    simpl. simpl in H1. apply andb_true_iff; split.
+    + apply O.leb_le. apply (O.le_trans _ t). apply O.leb_le. exact H.
+      apply O.leb_le. destruct (O.leb t a0); intuition.
+    + apply H0. rewrite andb_comm in H1. destruct (le_list t l0); intuition.
   Qed.
- *)
+
+  Lemma sorted_is_sorted : forall l, is_sorted l = true <-> sorted l.
+  Proof.
+    intros. elim l.
+    + intuition.
+    + intros. simpl. destruct l0.
+      - intuition.
+      - split.
+        * intro. constructor.
+          ++ simpl in H0. apply O.leb_le. destruct (O.leb a t); intuition.
+          ++ apply H. rewrite andb_comm in H0. destruct (is_sorted (t::l0)); intuition.
+        * intro. simpl. inversion H0. subst. apply andb_true_iff. split.
+          ++ apply andb_true_iff. split.
+            -- apply O.leb_le. exact H3.
+            -- apply (le_le_list _ t). apply O.leb_le. exact H3.
+               simpl in H. destruct (le_list t l0); intuition.
+          ++ apply H. exact H5.
+  Qed.
+
+  Lemma sort_is_sorted : forall l, is_sorted (sort l) = true.
+  Proof.
+    intros. apply sorted_is_sorted. apply sort_sorted.
+  Qed.
+
+  Lemma count_occ_insert_eq x bl :
+    count_occ O.eq_dec (insert x bl) x = S (count_occ O.eq_dec bl x).
+  Proof.
+    elim bl; intuition.
+    + simpl. destruct (O.eq_dec x x); intuition.
+    + simpl. destruct (O.leb x a); simpl; intuition.
+      - destruct (O.eq_dec x x); intuition.
+      - destruct (O.eq_dec a x); intuition.
+  Qed.
+
+  Lemma count_occ_insert_neq x y bl : x <> y ->
+    count_occ O.eq_dec (insert x bl) y = count_occ O.eq_dec bl y.
+  Proof.
+    intro. elim bl; intuition.
+    + simpl. destruct (O.eq_dec x y); intuition.
+    + simpl. destruct (O.leb x a); simpl; intuition.
+      - destruct (O.eq_dec x y); intuition.
+      - destruct (O.eq_dec a y); intuition.
+  Qed.
+
+  Lemma count_occ_insert : forall al bl x y, 
+    count_occ O.eq_dec al x = count_occ O.eq_dec bl x ->
+    count_occ O.eq_dec (y::al) x = count_occ O.eq_dec (insert y bl) x.
+  Proof.
+    intros. simpl. destruct (O.eq_dec y x).
+    - rewrite e. rewrite count_occ_insert_eq. rewrite H. reflexivity.
+    - erewrite count_occ_insert_neq; auto.
+  Qed.
+
+  Lemma count_occ_sort : forall al x, count_occ O.eq_dec al x = count_occ O.eq_dec (sort al) x.
+  Proof.
+    intros. elim al; intuition.
+    simpl (sort (a::l)). apply count_occ_insert. apply H.
+  Qed.
+
+  Theorem insertion_sort_correct:  is_a_sorting_algorithm sort.
+  Proof.
+    split.
+    + intro. apply count_occ_sort.
+    + apply sort_sorted.
+  Qed.
+
+  Lemma lt_sorted_count_occ_O a b l:
+    O.lt a b -> sorted (b::l) -> count_occ O.eq_dec (b::l) a = O.
+  Proof.
+    intros. generalize b H H0. clear b H H0. induction l; intros.
+    + simpl. destruct (O.eq_dec b a); intuition. 
+      rewrite e in H. destruct (O.lt_norefl _ H).
+    + inversion H0; intuition. simpl.
+      destruct (O.eq_dec b a); intuition.
+      - rewrite e in H. destruct (O.lt_norefl _ H).
+      - eapply (IHl a0).
+        * destruct (proj1 (O.le_lteq b a0) H3).
+          ++ apply (O.lt_trans _ _ _ H). exact H6.
+          ++ rewrite <- H6. exact H.
+        * exact H5.
+  Qed.
+
+  Theorem ext_eq al bl : 
+    sorted al -> sorted bl -> 
+    (forall x, count_occ O.eq_dec al x = count_occ O.eq_dec bl x) ->
+    al = bl.
+  Proof.
+    intros. generalize bl H0 H1. clear bl H0 H1. induction al; intros.
+
+    destruct bl; intuition. absurd (count_occ O.eq_dec [] t = count_occ O.eq_dec (t::bl) t).
+    simpl. destruct (O.eq_dec t t); intuition. discriminate H2.
+    apply H1.
+
+    destruct bl; intuition. absurd (count_occ O.eq_dec (a::al) a = count_occ O.eq_dec [] a).
+    simpl. destruct (O.eq_dec a a); intuition. discriminate H2.
+    apply H1.
+
+    destruct (O.linearity a t).
+    + subst. f_equal. assert (sorted al). inversion H; intuition.
+      assert (sorted bl). inversion H0; intuition.
+      apply IHal; intuition.
+      pose (H1' := H1 x); clearbody H1'. simpl in H1'. destruct (O.eq_dec t x); intuition.
+    + destruct H2.
+      - absurd (count_occ O.eq_dec (a::al) a = count_occ O.eq_dec (t::bl) a).
+        * rewrite (lt_sorted_count_occ_O _ _ _ H2 H0). simpl.
+          destruct (O.eq_dec a a); intuition. discriminate H3.
+        * apply H1.
+      - absurd (count_occ O.eq_dec (a::al) t = count_occ O.eq_dec (t::bl) t).
+        * rewrite (lt_sorted_count_occ_O _ _ _ H2 H). simpl.
+          destruct (O.eq_dec t t); intuition. discriminate H3.
+        * apply H1.
+  Qed.
 
 End InsertionSort.
